update finset

lemmas.lean
@@ -1,4 +1,4 @@
-import tools.super
+import tools.super .card
 open classical nat function set tactic
 
 section
@@ -6,12 +6,12 @@ section
 
 parameter {X : Type}
 
-theorem ext {a b : set X} (H : ∀x, x ∈ a ↔ x ∈ b) : a = b := funext (λ x, propext (H x))
+-- theorem ext {a b : set X} (H : ∀x, x ∈ a ↔ x ∈ b) : a = b := funext (λ x, propext (H x))
 
 theorem not_mem_empty (x : X) : ¬ (x ∈ (∅ : set X)) := λ H, H
 
 theorem eq_empty_of_forall_not_mem {s : set X} (H : ∀ x, x ∉ s) : s = ∅ :=
-ext (λ x, iff.intro (λ xs, absurd xs (H x)) (λ xe, absurd xe (not_mem_empty _)))
+set.ext (λ x, iff.intro (λ xs, absurd xs (H x)) (λ xe, absurd xe (not_mem_empty _)))
 
 theorem exists_mem_of_ne_empty {s : set X} (H : s ≠ ∅) : ∃ x, x ∈ s :=
 by_contradiction (λ H', H (eq_empty_of_forall_not_mem (forall_not_of_not_exists H')))
@@ -25,7 +25,7 @@ section
 def complete_induction_on (n : ℕ) {p : ℕ → Prop} (h : ∀ n, (∀ m < n, p m) → p n) : p n :=
 suffices ∀ n, ∀ m < n, p m, from this (succ n) _ (lt_succ_self n),
 take n,
-nat.induction_on n
+nat.rec_on n
   (take m, suppose m < 0, absurd this (not_lt_zero m))
   (take n,
     assume ih : ∀ m < n, p m,
@@ -36,13 +36,13 @@ nat.induction_on n
       (suppose m = n,
         begin rw this, apply h, exact ih end))
 
-lemma wf_aux {A : set ℕ} (n : ℕ) : n ∈ A → ∃ a ∈ A, ∀ b ∈ A, a ≤ b := 
-@complete_induction_on n (λ x, x ∈ A → ∃ a ∈ A, ∀ b ∈ A, a ≤ b)
+lemma wf_aux {A : set ℕ} (n : ℕ) : n ∈ A → ∃ a, a ∈ A ∧ ∀ b,  b ∈  A → a ≤ b := 
+@complete_induction_on n (λ x, x ∈ A → ∃ a, a ∈  A ∧ ∀ b, b ∈ A → a ≤ b)
 (λ k ih h, by_cases
-(suppose ∃ m ∈ A, m <k, let ⟨m, Hmem, Hlt⟩ := this in ih m Hlt Hmem)
-(λ Hn, have ∀ m ∈ A,  ¬ m < k, by super, ⟨k,h,(λ m h, le_of_not_gt $ this m h)⟩))
+(suppose ∃ m, m ∈ A ∧ m <k, let ⟨m, Hmem, Hlt⟩ := this in ih m Hlt Hmem)
+(λ Hn, have ∀ m, m ∈  A →  ¬ m < k, by super, ⟨k,h,(λ m h, le_of_not_gt $ this m h)⟩))
 
-theorem wf_of_le (S : set ℕ) (H : S ≠ ∅) : ∃ a ∈ S, ∀ b ∈ S, a ≤ b :=
+theorem wf_of_le (S : set ℕ) (H : S ≠ ∅) : ∃ a, a ∈ S ∧ ∀ b, b ∈ S → a ≤ b :=
 let ⟨n,Hn⟩ := exists_mem_of_ne_empty H in wf_aux n Hn
 
 noncomputable definition least (S : set ℕ) (H : S ≠ ∅) : ℕ := some (wf_of_le S H)
@@ -50,9 +50,7 @@ noncomputable definition least (S : set ℕ) (H : S ≠ ∅) : ℕ := some (wf_o
 theorem least_is_mem (S : set ℕ) (H : S ≠ ∅) : least S H ∈ S := 
 let ⟨bound, Ha⟩ := some_spec (wf_of_le S H) in bound
 
--- theorem minimality {S : set ℕ} {a : ℕ} {H0 : S ≠ ∅} (H : a = least S H0): 
-
-theorem minimality {S : set ℕ} {a : ℕ} {neq : S ≠ ∅}: ∀ x ∈ S, least S neq ≤ x := 
+theorem minimality {S : set ℕ} {a : ℕ} {neq : S ≠ ∅}: ∀ x, x ∈ S → least S neq ≤ x := 
 λ x Hx, let ⟨bound, Ha⟩ := some_spec (wf_of_le S neq) in Ha x Hx
 
 end
@@ -63,40 +61,42 @@ by_contradiction
 have card S = 0, from card_of_not_finite this,
 H this)
 
-lemma mem_not_in_diff {A : Type} {S : set A} {a : A} : a ∉ S \ '{a} := 
-suppose a ∈ S \ '{a},
-have a ∉ '{a}, from not_mem_of_mem_diff this,
+lemma mem_not_in_diff {A : Type} {S : set A} {a : A} : a ∉ S \ insert a (∅ : set A) := 
+assume h,
+have a ∉ insert a (∅ : set A), from not_mem_of_mem_diff h,
 this (mem_singleton a)
 
-lemma insert_of_diff_singleton {A : Type} {S : set A} {a : A} (H : a ∈ S) : insert a (S \ '{a}) = S :=
+lemma insert_of_diff_singleton {A : Type} {S : set A} {a : A} (H : a ∈ S) : insert a (S \ insert a (∅ : set A)) = S :=
 begin
 apply eq_of_subset_of_subset,
-  intros x h, apply or.elim h, intro, simp,
-  intro hr, apply and.left hr,
-  intro x h', cases (decidable.em (x ∈ '{a})),
-  apply or.inl, apply eq_of_mem_singleton, simp,
-  apply or.inr, apply and.intro, repeat simp
+intros x h, apply or.elim h, intro h1, simp [H, h1], -- simp,
+intro hr, apply and.left hr,
+intros x h', cases (decidable.em (x ∈ insert a (∅ : set A))),
+apply or.inl, apply eq_of_mem_singleton, assumption,
+apply or.inr, apply and.intro, repeat {assumption}
 end
 
-lemma union_of_diff_singleton {A : Type} {S : set A} {a : A} (H : a ∈ S) : S \ '{a} ∪ '{a} = S := 
-begin
-apply eq_of_subset_of_subset,
-  intros x h, apply or.elim h, intro hl, apply and.left hl,
-  intro hr, have x = a, from (and.left (mem_singleton_iff x a)) hr,
-  rewrite this, simp,
-  intros x h', cases (decidable.em (x ∈ '{a})),
-  apply or.inr, simp, apply or.inl, apply and.intro, repeat simp
-end
+-- lemma union_of_diff_singleton {A : Type} {S : set A} {a : A} (H : a ∈ S) 
+--   : S \ (insert a (∅ : set A)) ∪ (insert a (∅ : set A)) = S := 
+-- begin
+-- apply eq_of_subset_of_subset,
+--   intros x h, apply or.elim h, intro hl, apply and.left hl,
+--   intro hr, have h : x = a, from (mem_singleton_iff x a)^.mp hr,
+--   rewrite h, simp,
+--   intros x h', cases (decidable.em (x ∈ insert a (∅ : set A))),
+--   apply or.inr, simp, apply or.inl, apply and.intro, repeat {simp}
+-- end
 
-lemma finite_singleton {A : Type} {a : A} : finite '{a} := 
-have carda : card '{a} = 1, from card_singleton a,
-have (1:ℕ) ≠ 0, from dec_trivial,
-have card '{a} ≠ 0, by+ rewrite -carda at this;exact this,
-nonzero_card_of_finite this
 
-lemma sub_of_eq {A : Type} {S T: set A} (H : S = T) : S ⊆ T :=
-have T ⊆ T, from subset.refl T,
-by+ rewrite -H at this{1};exact this
+-- lemma finite_singleton {A : Type} {a : A} : finite '{a} := 
+-- have carda : card '{a} = 1, from card_singleton a,
+-- have (1:ℕ) ≠ 0, from dec_trivial,
+-- have card '{a} ≠ 0, by+ rewrite -carda at this;exact this,
+-- nonzero_card_of_finite this
 
-theorem ne_empty_of_mem' {X : Type} {s : set X} {x : X} (H : x ∈ s) : s ≠ ∅ :=
-begin intro Hs, rewrite Hs at H, apply not_mem_empty _ H end --this is on github
+-- lemma sub_of_eq {A : Type} {S T: set A} (H : S = T) : S ⊆ T :=
+-- have T ⊆ T, from subset.refl T,
+-- by+ rewrite -H at this{1};exact this
+
+-- theorem ne_empty_of_mem' {X : Type} {s : set X} {x : X} (H : x ∈ s) : s ≠ ∅ :=
+-- begin intro Hs, rewrite Hs at H, apply not_mem_empty _ H end --this is on github
