finite.lean
@@ -10,10 +10,10 @@ noncomputable instance type_decidable_eq (A : Type) : decidable_eq A :=
 namespace set
 
 attribute [class]
-definition finite (s : set A) : Prop := ∃ (s' : finset A), s = ↑s'
+definition finite (s : set A) : Prop := ∃ (s' : finset A), s = finset.to_set s'
 
 attribute [instance]
-theorem finite_finset (s : finset A) : finite (finset.to_set s) :=
+definition finite_finset (s : finset A) : finite (finset.to_set s) :=
 exists.intro s rfl
 
 noncomputable instance dec_finite (s : set A) : decidable (finite s) := prop_decidable (finite s)
@@ -24,26 +24,26 @@ if fins : finite s then some fins else finset.empty
 theorem to_finset_of_not_finite {s : set A} (nfins : ¬ finite s) : to_finset s = finset.empty := 
 dif_neg nfins
 
-theorem to_set_to_finset (s : set A) [fins : finite s] : ↑(to_finset s) = s :=
+theorem to_set_to_finset (s : set A) [fins : finite s] : finset.to_set (to_finset s) = s :=
 have to_finset s = some fins, from dif_pos fins,
 by rw this; exact eq.symm (some_spec fins)
 
--- theorem mem_to_finset_eq (a : A) (s : set A) [finite s] :
---   (#finset a ∈ to_finset s) = (a ∈ s) :=
--- by rewrite [-to_set_to_finset at {2}]
+theorem mem_to_finset_eq (a : A) (s : set A) [finite s] :
+  (finset.mem a (to_finset s)) = (a ∈ s) :=
+have (finset.mem a (to_finset s)) = (a ∈ (finset.to_set (to_finset s))), from rfl,
+begin rw this, rw [to_set_to_finset] end
 
 theorem to_set_to_finset_of_not_finite {s : set A} (nfins : ¬ finite s) :
   finset.to_set (to_finset s) = ∅ :=
 have to_finset s = finset.empty, from to_finset_of_not_finite nfins,
 begin rw this, reflexivity end
 
--- theorem to_finset_to_set (s : finset A) : to_finset (finset.to_set s) = s :=
--- by rewrite [finset.eq_eq_to_set_eq, to_set_to_finset (finset.to_set s)]
+theorem to_finset_to_set (s : finset A) : to_finset (finset.to_set s) = s :=
+begin rw finset.eq_eq_to_set_eq, rw to_set_to_finset end
 
--- theorem to_finset_eq_of_to_set_eq {s : set A} {t : finset A} (H : finset.to_set t = s) :
---   to_finset s = t :=
--- finset.eq_of_to_set_eq_to_set (by subst [s]; rewrite to_finset_to_set)
-
+theorem to_finset_eq_of_to_set_eq {s : set A} {t : finset A} (H : finset.to_set t = s) :
+  to_finset s = t :=
+finset.eq_of_to_set_eq_to_set (begin rw -H, rw to_finset_to_set end)
 
 theorem finite_of_to_set_to_finset_eq {s : set A} (H : finset.to_set (to_finset s) = s) :
   finite s :=
@@ -53,16 +53,171 @@ attribute [instance]
 theorem finite_empty : finite (∅ : set A) :=
 by rewrite [-finset.to_set_empty]; apply finite_finset
 
+theorem to_finset_empty : to_finset (∅ : set A) = finset.empty :=
+to_finset_eq_of_to_set_eq finset.to_set_empty
+
+theorem to_finset_eq_empty_of_eq_empty {s : set A} [fins : finite s] (H : s = ∅) :
+  to_finset s = finset.empty := by rewrite [H, to_finset_empty]
+
+theorem eq_empty_of_to_finset_eq_empty {s : set A} [fins : finite s]
+    (H : to_finset s = finset.empty) :
+s = ∅ := by rewrite [-finset.to_set_empty, -H, to_set_to_finset]
+
+theorem to_finset_eq_empty (s : set A) [fins : finite s] :
+  (to_finset s = finset.empty) ↔ (s = ∅) :=
+iff.intro eq_empty_of_to_finset_eq_empty to_finset_eq_empty_of_eq_empty
+
 attribute [instance]
 theorem finite_insert (a : A) (s : set A) [finite s] : finite (set.insert a s) :=
 exists.intro (finset.insert a (to_finset s))
-(begin rw [-finset.to_set_insert, to_set_to_finset], end)
+(by rw [-(to_set_to_finset s), finset.to_set_insert, to_finset_to_set])
+
+theorem to_finset_insert (a : A) (s : set A) [finite s] :
+  to_finset (insert a s) = finset.insert a (to_finset s) :=
+begin apply to_finset_eq_of_to_set_eq, 
+rw [-finset.to_set_insert, to_set_to_finset], reflexivity end
+
+attribute [instance]
+theorem finite_union (s t : set A) [finite s] [finite t] :
+  finite (s ∪ t) :=
+exists.intro (to_finset s ∪ to_finset t)
+(by rewrite [finset.to_set_union]; repeat {rw to_set_to_finset})
+
+theorem to_finset_union (s t : set A) [finite s] [finite t] :
+  to_finset (s ∪ t) = (to_finset s ∪ to_finset t) :=
+by apply to_finset_eq_of_to_set_eq; rw [finset.to_set_union]; repeat {rw to_set_to_finset}
+
+attribute [instance]
+theorem finite_inter (s t : set A) [finite s] [finite t] :
+  finite (s ∩ t) :=
+exists.intro (to_finset s ∩ to_finset t)
+(by rw [finset.to_set_inter]; repeat {rw to_set_to_finset})
+
+theorem to_finset_inter (s t : set A) [finite s] [finite t] :
+  to_finset (s ∩ t) = (to_finset s ∩ to_finset t) :=
+by apply to_finset_eq_of_to_set_eq; rw [finset.to_set_inter]; repeat {rw to_set_to_finset}
+
+noncomputable instance dec_prop (p : Prop) : decidable p := prop_decidable p
+
+attribute [instance]
+theorem finite_sep (s : set A) (p : A → Prop) [finite s] :
+  finite {x ∈ s | p x}  :=
+exists.intro (finset.sep p (to_finset s))
+(by rw [finset.to_set_sep]; rw to_set_to_finset; reflexivity)
+
+theorem to_finset_sep (s : set A) (p : A → Prop) [finite s] :
+  to_finset {x ∈ s | p x} = finset.sep p (to_finset s) :=
+begin apply to_finset_eq_of_to_set_eq; rewrite [finset.to_set_sep, to_set_to_finset], reflexivity end
+
+attribute [instance]
+theorem finite_image {B : Type} (f : A → B) (s : set A) [finite s] :
+  finite (image f s) :=
+exists.intro (finset.image f (to_finset s))
+(begin rw [finset.to_set_image]; repeat {rw to_set_to_finset} end)
+
+theorem to_finset_image {B : Type}  (f : A → B) (s : set A)
+    [fins : finite s] :
+  to_finset (image f s) = (finset.image f (to_finset s)) :=
+by apply to_finset_eq_of_to_set_eq; rewrite [finset.to_set_image, to_set_to_finset]
+
+attribute [instance]
+theorem finite_diff (s t : set A) [finite s] : finite (s \ t) :=
+finite_sep _ _
+
+theorem to_finset_diff (s t : set A) [finite s] [finite t] :
+        to_finset (s \ t) = (to_finset s \ to_finset t) :=
+by apply to_finset_eq_of_to_set_eq; rw [finset.to_set_diff]; repeat {rw to_set_to_finset}
+
+theorem finite_subset {s t : set A} [finite t] (ssubt : s ⊆ t) : finite s :=
+by rewrite (eq_sep_of_subset ssubt); apply finite_sep
+
+theorem to_finset_subset_to_finset_eq (s t : set A) [finite s] [finite t] :
+  (to_finset s ⊆ to_finset t) = (s ⊆ t) :=
+by rw [finset.subset_eq_to_set_subset]; repeat {rw to_set_to_finset}
+
+theorem finite_of_finite_insert {s : set A} {a : A} (finias : finite (insert a s)) : finite s :=
+finite_subset (subset_insert a s)
+
+attribute [instance]
+theorem finite_upto (n : ℕ) : finite {i | i < n} :=
+by rewrite [-finset.to_set_upto n]; apply finite_finset
+
+theorem to_finset_upto (n : ℕ) : to_finset {i | i < n} = finset.upto n :=
+by apply (to_finset_eq_of_to_set_eq (finset.to_set_upto _))
+
+theorem finite_of_surj_on {B : Type} {f : A → B} {s : set A} [finite s] {t : set B}
+                          (H : surj_on f s t) :
+        finite t :=
+finite_subset H
+
+theorem finite_of_inj_on {B : Type} {f : A → B} {s : set A} {t : set B} [finite t]
+                         (mapsto : maps_to f s t) (injf : inj_on f s) :
+        finite s :=
+if H : s = ∅ then
+  begin rewrite H; apply _, apply finite_empty end
+else
+  let ⟨dflt,xs⟩ := exists_mem_of_ne_empty H in
+  let finv := inv_fun f s dflt in
+  have surj_on finv t s, from surj_on_inv_fun_of_inj_on dflt mapsto injf,
+  finite_of_surj_on this
+
+-- theorem finite_of_bij_on {B : Type} {f : A → B} {s : set A} {t : set B} [finite s]
+--                          (bijf : bij_on f s t) :
+--         finite t :=
+-- finite_of_surj_on (surj_on_of_bij_on bijf)
+
+-- theorem finite_of_bij_on' {B : Type} {f : A → B} {s : set A} {t : set B} [finite t]
+--                          (bijf : bij_on f s t) :
+--         finite s :=
+-- finite_of_inj_on (maps_to_of_bij_on bijf) (inj_on_of_bij_on bijf)
+
+-- theorem finite_iff_finite_of_bij_on {B : Type} {f : A → B} {s : set A} {t : set B}
+--                                     (bijf : bij_on f s t) :
+--         finite s ↔ finite t :=
+-- iff.intro (assume fs, finite_of_bij_on bijf) (assume ft, finite_of_bij_on' bijf)
+
+-- theorem finite_powerset (s : set A) [finite s] : finite 𝒫 s :=
+-- have H : 𝒫 s = finset.to_set ' (finset.to_set (#finset 𝒫 (to_finset s))),
+--   from ext (take t, iff.intro
+--     (suppose t ∈ 𝒫 s,
+--       have t ⊆ s, from this,
+--       have finite t, from finite_subset this,
+--       have (#finset to_finset t ∈ 𝒫 (to_finset s)),
+--         by rewrite [finset.mem_powerset_iff_subset, to_finset_subset_to_finset_eq]; apply `t ⊆ s`,
+--       have to_finset t ∈ (finset.to_set (finset.powerset (to_finset s))), from this,
+--       mem_image this (by rewrite to_set_to_finset))
+--     (assume H',
+--       obtain t' [(tmem : (#finset t' ∈ 𝒫 (to_finset s))) (teq : finset.to_set t' = t)],
+--         from H',
+--       show t ⊆ s,
+--       begin
+--         rewrite [-teq, finset.mem_powerset_iff_subset at tmem, -to_set_to_finset s],
+--         rewrite -finset.subset_eq_to_set_subset, assumption
+--      end)),
+-- by rewrite H; apply finite_image
 
 
--- attribute [instance]
--- theorem finite_union (s t : set A) [finite s] [finite t] :
---   finite (s ∪ t) :=
--- exists.intro (to_finset s ∪ to_finset t)
--- (begin  end)
+/- induction for finite sets -/
+
+attribute [recursor 6]
+theorem induction_finite {P : set A → Prop}
+    (H1 : P ∅) (H2 : ∀ ⦃a : A⦄, ∀ {s : set A} [finite s], a ∉ s → P s → P (insert a s)) :
+  ∀ (s : set A) [finite s], P s :=
+(λ s fins, 
+have ∀ s' : finset A, P (finset.to_set s'), from 
+  λ s', @finset.induction_on _ _ (λ x, P (finset.to_set x)) s' 
+  (by rw finset.to_set_empty; exact H1) 
+  (begin 
+    intros a s' anin ih, 
+    rw [-finset.to_set_insert], apply H2, 
+    {rw [-finset.mem_eq_mem_to_set], exact anin},
+    {exact ih} 
+   end),
+begin rw [-to_set_to_finset s], exact (this (to_finset s)) end)
+
+theorem induction_on_finite {P : set A → Prop} (s : set A) [finite s]
+    (H1 : P ∅) (H2 : ∀ ⦃a : A⦄, ∀ {s : set A} [finite s], a ∉ s → P s → P (insert a s)) :
+  P s :=
+induction_finite H1 H2 s
 
 end set
