finset/misc.lean
@@ -1,6 +1,212 @@
-open nat
+open nat set
 
 theorem lt_succ_iff_le (m n : nat) : m < succ n ↔ m ≤ n :=
 iff.intro le_of_lt_succ lt_succ_of_le
 
-#check lt_succ_iff_le
+theorem ext {X : Type} {a b : set X} (H : ∀x, x ∈ a ↔ x ∈ b) : a = b :=
+funext (take x, propext (H x))
+
+theorem not_mem_empty {X : Type} (x : X) : ¬ (x ∈ (∅ : set X)) :=
+assume H : x ∈ ∅, H
+
+section 
+/- universal set -/
+variable {α : Type}
+
+theorem mem_univ (x : α) : x ∈ @univ α := trivial
+
+theorem mem_univ_iff (x : α) : x ∈ @univ α ↔ true := iff.rfl
+
+@[simp]
+theorem mem_univ_eq (x : α) : x ∈ @univ α = true := rfl
+
+theorem empty_ne_univ [h : inhabited α] : (∅ : set α) ≠ univ :=
+assume H : ∅ = univ,
+absurd (mem_univ (inhabited.default α)) (eq.rec_on H (not_mem_empty _))
+
+@[simp]
+theorem subset_univ (s : set α) : s ⊆ univ := λ x H, trivial
+
+end
+
+
+theorem eq_sep_of_subset {X : Type} {s t : set X} (ssubt : s ⊆ t) : s = {x ∈ t | x ∈ s} :=
+ext (take x, iff.intro
+  (suppose x ∈ s, and.intro (ssubt this) this)
+(suppose x ∈ {x ∈ t | x ∈ s}, and.right this))
+
+theorem subset_insert {X : Type} (x : X) (a : set X) : a ⊆ insert x a :=
+take y, assume ys, or.inr ys
+
+theorem not_mem_of_mem_diff {A : Type} {s t : set A} {x : A} (H : x ∈ s \ t) : x ∉ t :=
+and.right H
+
+theorem mem_insert {X : Type} (x : X) (s : set X) : x ∈ insert x s :=
+or.inl rfl
+
+theorem mem_singleton {X : Type} (a : X) : a ∈ insert a (∅ : set X) := mem_insert _ _
+
+theorem eq_of_mem_singleton {X : Type} {x y : X} (h : x ∈ insert y (∅ : set X)) : x = y :=
+or.elim (h)
+  (suppose x = y, this)
+(suppose x ∈ ∅, absurd this (not_mem_empty _))
+
+theorem mem_singleton_iff {X : Type} (a b : X) : a ∈ insert b (∅ : set X) ↔ a = b :=
+iff.intro
+  (assume ainb, or.elim ainb (λ aeqb, aeqb) (λ f, false.elim f))
+(assume aeqb, or.inl aeqb)
+
+theorem eq_empty_of_forall_not_mem {X : Type} {s : set X} (H : ∀ x, x ∉ s) : s = ∅ :=
+ext (take x, iff.intro
+  (assume xs, absurd xs (H x))
+(assume xe, absurd xe (not_mem_empty _)))
+
+section
+  open classical
+  variable {X : Type}
+
+  theorem exists_mem_of_ne_empty {s : set X} (H : s ≠ ∅) : ∃ x, x ∈ s :=
+  by_contradiction (assume H', H (eq_empty_of_forall_not_mem (forall_not_of_not_exists H')))
+
+end
+
+definition eq_on {X Y : Type} (f1 f2 : X → Y) (a : set X) : Prop :=
+∀ x ∈ a, f1 x = f2 x
+
+attribute [reducible]
+definition maps_to {X Y : Type} (f : X → Y) (a : set X) (b : set Y) : Prop := ∀⦃x⦄, x ∈ a → f x ∈ b
+
+
+attribute [reducible]
+definition surj_on {X Y : Type} (f : X → Y) (a : set X) (b : set Y) : Prop := b ⊆ image f a
+
+attribute [reducible]
+definition inj_on {X Y: Type} (f : X → Y) (a : set X) : Prop :=
+∀⦃x1 x2 : X⦄, x1 ∈ a → x2 ∈ a → f x1 = f x2 → x1 = x2
+
+section function
+
+variables {X Y Z: Type}
+/- left inverse -/
+
+-- g is a left inverse to f on a
+attribute [reducible]
+definition left_inv_on  (g : Y → X) (f : X → Y) (a : set X) : Prop :=
+∀ x ∈ a, g (f x) = x
+
+theorem left_inv_on_of_eq_on_left {g1 g2 : Y → X} {f : X → Y} {a : set X} {b : set Y}
+  (fab : maps_to f a b) (eqg : eq_on g1 g2 b) (H : left_inv_on g1 f a) : left_inv_on g2 f a :=
+take x,
+assume xa : x ∈ a,
+calc
+  g2 (f x) = g1 (f x) : eq.symm (eqg _ (fab xa))
+  ... = x : H _ xa
+
+theorem left_inv_on_of_eq_on_right {g : Y → X} {f1 f2 : X → Y} {a : set X}
+  (eqf : eq_on f1 f2 a) (H : left_inv_on g f1 a) : left_inv_on g f2 a :=
+take x,
+assume xa : x ∈ a,
+calc
+  g (f2 x) = g (f1 x) : by rw eq.symm (eqf _ xa)
+... = x : H _ xa
+
+theorem inj_on_of_left_inv_on {g : Y → X} {f : X → Y} {a : set X} (H : left_inv_on g f a) :
+  inj_on f a :=
+take x1 x2,
+assume x1a : x1 ∈ a,
+assume x2a : x2 ∈ a,
+assume H1 : f x1 = f x2,
+calc
+  x1     = g (f x1) : eq.symm (H _ x1a)
+     ... = g (f x2) : by rw H1
+     ... = x2 : H _ x2a
+
+theorem left_inv_on_comp {f' : Y → X} {g' : Z → Y} {g : Y → Z} {f : X → Y}
+   {a : set X} {b : set Y} (fab : maps_to f a b)
+    (Hf : left_inv_on f' f a) (Hg : left_inv_on g' g b) : left_inv_on (f' ∘ g') (g ∘ f) a :=
+take x : X,
+assume xa : x ∈ a,
+have fxb : f x ∈ b, from fab xa,
+calc
+  f' (g' (g (f x))) = f' (f x) : by rw Hg _ fxb
+  ... = x : Hf _ xa
+
+
+/- right inverse -/
+
+-- g is a right inverse to f on a
+attribute [reducible]
+definition right_inv_on (g : Y → X) (f : X → Y) (b : set Y) : Prop :=
+left_inv_on f g b
+
+theorem right_inv_on_of_eq_on_left {g1 g2 : Y → X} {f : X → Y} {a : set X} {b : set Y}
+  (eqg : eq_on g1 g2 b) (H : right_inv_on g1 f b) : right_inv_on g2 f b :=
+left_inv_on_of_eq_on_right eqg H
+
+theorem right_inv_on_of_eq_on_right {g : Y → X} {f1 f2 : X → Y} {a : set X} {b : set Y}
+  (gba : maps_to g b a) (eqf : eq_on f1 f2 a) (H : right_inv_on g f1 b) : right_inv_on g f2 b :=
+left_inv_on_of_eq_on_left gba eqf H
+
+theorem surj_on_of_right_inv_on {g : Y → X} {f : X → Y} {a : set X} {b : set Y}
+    (gba : maps_to g b a) (H : right_inv_on g f b) :
+  surj_on f a b :=
+take y,
+assume yb : y ∈ b,
+have gya : g y ∈ a, from gba yb,
+have H1 : f (g y) = y, from H _ yb,
+exists.intro (g y) (and.intro gya H1)
+
+
+end function
+
+section
+
+-- classical inverse
+
+open classical
+variables {X Y : Type}
+
+noncomputable instance dec_prop (p : Prop) : decidable p := prop_decidable p
+
+noncomputable definition inv_fun (f : X → Y) (a : set X) (dflt : X) (y : Y) : X :=
+if H : ∃ x ∈ a, f x = y then some H else dflt
+
+theorem inv_fun_pos {f : X → Y} {a : set X} {dflt : X} {y : Y}
+  (H : ∃ x ∈ a, f x = y) : (inv_fun f a dflt y ∈ a) ∧ (f (inv_fun f a dflt y) = y) :=
+have H1 : inv_fun f a dflt y = some H, from dif_pos H,
+let ⟨x,ina⟩ := some_spec H in
+⟨by rw H1; assumption,by rw H1; assumption⟩
+
+theorem inv_fun_neg {f : X → Y} {a : set X} {dflt : X} {y : Y}
+  (H : ¬ ∃ x ∈ a, f x = y) : inv_fun f a dflt y = dflt :=
+dif_neg H
+
+variables {f : X → Y} {a : set X} {b : set Y}
+
+theorem maps_to_inv_fun {dflt : X} (dflta : dflt ∈ a) :
+  maps_to (inv_fun f a dflt) b a :=
+let f' := inv_fun f a dflt in
+take y,
+assume yb : y ∈ b,
+show f' y ∈ a, from
+  by_cases
+    (assume H : ∃ x ∈ a, f x = y,
+      and.left (inv_fun_pos H))
+    (assume H : ¬ ∃ x ∈ a, f x = y,
+begin dsimp, rw (inv_fun_neg H), assumption end)
+
+theorem left_inv_on_inv_fun_of_inj_on (dflt : X) (H : inj_on f a) :
+  left_inv_on (inv_fun f a dflt) f a :=
+let f' := inv_fun f a dflt in
+take x,
+assume xa : x ∈ a,
+have H1 : ∃ x' ∈ a, f x' = f x, from ⟨x,xa,rfl⟩,
+have H2 : f' (f x) ∈ a ∧ f (f' (f x)) = f x, from inv_fun_pos H1,
+show f' (f x) = x, from H (and.left H2) xa (and.right H2)
+
+theorem surj_on_inv_fun_of_inj_on (dflt : X) (mapsto : maps_to f a b) (H : inj_on f a) :
+  surj_on (inv_fun f a dflt) b a :=
+surj_on_of_right_inv_on mapsto (left_inv_on_inv_fun_of_inj_on dflt H)
+
+
+end
