finset/to_set.lean
@@ -8,76 +8,75 @@ variable [deceq : decidable_eq A]
 
 definition to_set (s : finset A) : set A := λx, x ∈ s
 
-def ts := @to_set A
-instance finset_to_set_coe : has_coe (finset A) (set A) := ⟨ts⟩
+-- def ts := @to_set A
+instance finset_to_set_coe : has_coe (finset A) (set A) := ⟨to_set⟩
 
 variables (s t : finset A) (x y : A)
 
-theorem mem_eq_mem_to_set : x ∈ s = (x ∈ ts s) := rfl
+theorem mem_eq_mem_to_set : x ∈ s = (x ∈ to_set s) := rfl
 
-definition to_set.inj {s₁ s₂ : finset A} : ts s₁ = ts s₂ → s₁ = s₂ :=
+definition to_set.inj {s₁ s₂ : finset A} : to_set s₁ = to_set s₂ → s₁ = s₂ :=
 λ h, ext (λ a, iff.of_eq (calc
-  (a ∈ s₁) = (a ∈ ts s₁) : mem_eq_mem_to_set _ _
-       ... = (a ∈ ts s₂) : by rw -h
+  (a ∈ s₁) = (a ∈ to_set s₁) : mem_eq_mem_to_set _ _
+       ... = (a ∈ to_set s₂) : by rw -h
        ... = (a ∈ s₂) : mem_eq_mem_to_set _ _))
 
 -- A example
-theorem mem_to_set_empty : (set.mem x (ts empty)) = (mem x empty) := rfl
-theorem to_set_empty : ts empty = (∅:set A) := rfl
+theorem mem_to_set_empty : (set.mem x (to_set empty)) = (mem x empty) := rfl
+theorem to_set_empty : to_set empty = (∅:set A) := rfl
 
--- theorem mem_to_set_univ [h : fintype A] : (x ∈ ts univ) = (x ∈ set.univ) :=
+-- theorem mem_to_set_univ [h : fintype A] : (x ∈ to_set univ) = (x ∈ set.univ) :=
 --   propext (iff.intro (assume H, trivial) (assume H, !mem_univ))
--- theorem to_set_univ [h : fintype A] : ts univ = (set.univ : set A) := funext (λ x, !mem_to_set_univ)
+-- theorem to_set_univ [h : fintype A] : to_set univ = (set.univ : set A) := funext (λ x, !mem_to_set_univ)
 
 -- instance : has_subset (finset A) := ⟨finset.subset⟩
 
-theorem mem_to_set_upto (x n : ℕ) : x ∈ ts (upto n) = (x ∈ {a | a < n}) := mem_upto_eq _ _
-theorem to_set_upto (n : ℕ) : ts (upto n) = {a | a < n} := funext (λ x, mem_to_set_upto _ _)
+theorem mem_to_set_upto (x n : ℕ) : x ∈ to_set (upto n) = (x ∈ {a | a < n}) := mem_upto_eq _ _
+theorem to_set_upto (n : ℕ) : to_set (upto n) = {a | a < n} := funext (λ x, mem_to_set_upto _ _)
 
 include deceq
 
 theorem mem_to_set_insert : x ∈ insert y s = (x ∈ set.insert y s) := mem_insert_eq _ _ _
 
-theorem to_set_insert : (set.insert y s) = (insert y s) := funext (λ x, eq.symm (mem_to_set_insert _ _ _))
+theorem to_set_insert : (set.insert y (to_set s)) = to_set (insert y s) := funext (λ x, eq.symm (mem_to_set_insert _ _ _))
 
-theorem mem_to_set_union : x ∈ s ∪ t = (x ∈ ts s ∪ ts t) := mem_union_eq _ _ _
-theorem to_set_union : ts (s ∪ t) = ts s ∪ ts t := funext (λ x, mem_to_set_union _ _ _)
+theorem mem_to_set_union : x ∈ s ∪ t = (x ∈ to_set s ∪ to_set t) := mem_union_eq _ _ _
+theorem to_set_union : to_set (s ∪ t) = to_set s ∪ to_set t := funext (λ x, mem_to_set_union _ _ _)
 
-theorem mem_to_set_inter : x ∈ s ∩ t = (x ∈ ts s ∩ ts t) := mem_inter_eq _ _ _
-theorem to_set_inter : ts (s ∩ t) = ts s ∩ ts t := funext (λ x, mem_to_set_inter _ _ _)
+theorem mem_to_set_inter : x ∈ s ∩ t = (x ∈ to_set s ∩ to_set t) := mem_inter_eq _ _ _
+theorem to_set_inter : to_set (s ∩ t) = to_set s ∩ to_set t := funext (λ x, mem_to_set_inter _ _ _)
 
-theorem mem_to_set_diff : x ∈ s \ t = (x ∈ ts s \ ts t) := mem_diff_eq _ _ _
-theorem to_set_diff : ts (s \ t) = ts s \ ts t := funext (λ x, mem_to_set_diff _ _ _)
-
+theorem mem_to_set_diff : x ∈ s \ t = (x ∈ to_set s \ to_set t) := mem_diff_eq _ _ _
+theorem to_set_diff : to_set (s \ t) = to_set s \ to_set t := funext (λ x, mem_to_set_diff _ _ _)
 
 theorem mem_to_set_sep (p : A → Prop) [h : decidable_pred p] : x ∈ sep p s = (x ∈ set.sep p s) :=
   finset.mem_sep_eq _ _
-theorem to_set_sep (p : A → Prop) [h : decidable_pred p] : ↑(sep p s) = set.sep p s :=
+theorem to_set_sep (p : A → Prop) [h : decidable_pred p] : to_set (sep p s) = set.sep p (to_set s) :=
   funext (λ x, mem_to_set_sep _ _ _)
 
 theorem mem_to_set_image {B : Type} [h : decidable_eq B] (f : A → B) {s : finset A} {y : B} :
   y ∈ image f s = (y ∈ set.image f s) := mem_image_eq _ 
 theorem to_set_image {B : Type} [h : decidable_eq B] (f : A → B) (s : finset A) :
-↑(image f s) = set.image f s := funext (λ x, mem_to_set_image _)
+to_set (image f s) = set.image f (to_set s) := funext (λ x, mem_to_set_image _)
 
 
 /- relations -/
 
 attribute [instance]
-definition decidable_mem_to_set (x : A) (s : finset A) : decidable (x ∈ ts s) :=
+definition decidable_mem_to_set (x : A) (s : finset A) : decidable (x ∈ to_set s) :=
 decidable_of_decidable_of_eq (decidable_mem _ _) (mem_eq_mem_to_set _ _)
 
-theorem eq_of_to_set_eq_to_set {s t : finset A} (H : ts s =  ts t) : s = t :=
+theorem eq_of_to_set_eq_to_set {s t : finset A} (H : to_set s =  to_set t) : s = t :=
 to_set.inj H
 
-theorem eq_eq_to_set_eq : (s = t) = (ts s = ts t) :=
+theorem eq_eq_to_set_eq : (s = t) = (to_set s = to_set t) :=
 propext (iff.intro (assume H, H ▸ rfl) eq_of_to_set_eq_to_set)
 
 attribute [instance]
-definition decidable_to_set_eq (s t : finset A) : decidable (ts s = ts t) :=
+definition decidable_to_set_eq (s t : finset A) : decidable (to_set s = to_set t) :=
 decidable_of_decidable_of_eq (has_decidable_eq _ _) (eq_eq_to_set_eq _ _)
 
-theorem subset_eq_to_set_subset (s t : finset A) : (s ⊆ t) = (ts s ⊆ ts t) :=
+theorem subset_eq_to_set_subset (s t : finset A) : (s ⊆ t) = (to_set s ⊆ to_set t) :=
 propext (iff.intro
   (assume H, take x xs, mem_of_subset_of_mem H xs)
   (assume H, subset_of_forall H))
@@ -86,23 +85,23 @@ propext (iff.intro
 -- definition decidable_subset [h : decidable_eq A] : ∀ (s t: finset A), decidable (s ⊆ t) :=
 -- sorry
 
--- definition decidable_to_set_subset (s t : finset A) : decidable (ts s ⊆ ts t) :=
+-- definition decidable_to_set_subset (s t : finset A) : decidable (to_set s ⊆ to_set t) :=
 -- decidable_of_decidable_of_eq (decidable_subset _ _) (subset_eq_to_set_subset _ _)
 
 /- bounded quantifiers -/
 
 -- definition decidable_bounded_forall (s : finset A) (p : A → Prop) [h : decidable_pred p] :
---   decidable (∀ x ∈ ts s, p x) :=
+--   decidable (∀ x ∈ to_set s, p x) :=
 -- decidable_of_decidable_of_iff _ !all_iff_forall
 
--- definition decidable_bounded_exists (s : finset A) (p : A → Prop) [h : decidable_pred p] :
---   decidable (∃₀ x ∈ ts s, p x) :=
+-- definition decidable_bounded_existo_set (s : finset A) (p : A → Prop) [h : decidable_pred p] :
+--   decidable (∃₀ x ∈ to_set s, p x) :=
 -- decidable_of_decidable_of_iff _ !any_iff_exists
 
 /- properties -/
 
 -- theorem inj_on_to_set {B : Type} [h : decidable_eq B] (f : A → B) (s : finset A) :
---   inj_on f s = inj_on f (ts s) :=
+--   inj_on f s = inj_on f (to_set s) :=
 -- rfl
 
 end finset
