test.lean
@@ -1,0 +1,19 @@
+structure quasiorder (A : Type) extends has_le A :=
+(refl : ∀ a, le a a)
+(trans : ∀ {a b c}, le a b → le b c → le a c)
+
+structure wqo (A : Type) extends quasiorder A :=
+(is_good : ∀ f : ℕ → A, ∃ i j : ℕ, i < j ∧ le (f i) (f j))
+
+-- the following works but the above does no.t
+
+-- variable {A : Type}
+
+-- structure has_refl (R : A → A → Prop) : Prop :=
+-- (refl : ∀ a, R a a)
+
+-- structure is_equiv (R : A → A → Prop) extends has_refl R : Prop :=
+-- (symm : ∀ a b, R a b → R b a)
+-- (trans : ∀ a b c, R a b → R b c → R a c)
+
+-- structure is_g (R : A → A → Prop) extends is_equiv R : Prop
